GenericPipeline/ProcessorCoreWellFormed.v
@@ -464,19 +464,14 @@ Proof.
     elim H.
     elim H1.
     intros.
-    repeat (decide equality).
+    apply string_dec.
 Qed.
 
 Theorem DisjKey_getAllRegisters_intRegFile_memReservationRegFile:
   DisjKey (getAllRegisters (BaseRegFile intRegFile))
     (getAllRegisters (BaseRegFile memReservationRegFile)).
 Proof.
-    unfold intRegFile.
-    unfold memReservationRegFile.
-    unfold getAllRegisters.
-    unfold getRegisters.
-    unfold getRegFileRegisters.
-    DisjKey_solve.
+    discharge_DisjKey.
 Qed.
 
 Theorem DisjKey_getAllRegisters_intRegFile_mem_devices:
@@ -528,18 +523,74 @@ Hint Resolve DisjKey_getAllRegisters_intRegFile_mem_device_regs_mem_devices : wf
 Theorem DisjKey_getAllRegisters_intRegFile_debug_internal_regs:
   DisjKey (getAllRegisters (BaseRegFile intRegFile)) debug_internal_regs.
 Proof.
-  unfold intRegFile.
-  unfold debug_internal_regs.
-  autorewrite with kami_rewrite_db.
-  autorewrite with simp_csrs.
-  simpl.
-  DisjKey_solve.
-  repeat (decide equality).
-  repeat (decide equality).
-  repeat (decide equality).
+  discharge_DisjKey.
 Qed.
 
 Hint Resolve DisjKey_getAllRegisters_intRegFile_debug_internal_regs : wfMod_ConcatMod_Helper.
+
+Theorem string_append_assoc: forall a b c, ((a++b)++c)%string=(a++(b++c))%string.
+Proof.
+    induction a.
+    + simpl.
+      reflexivity.
+    + intros.
+      simpl.
+      rewrite IHa.
+      reflexivity.
+Qed.
+
+Theorem string_glue: forall x y, (x++(String "_" y))%string=(x++"_"++y)%string.
+Proof.
+    intros.
+    simpl.
+    reflexivity.
+Qed.
+
+(*Theorem debug_csr_data_disjoint: forall x n,
+  In x%string (map fst (concat (map csr_reg_csr_field (concat (map csrViewFields (csrViews (Debug.debug_csr_data n))))))) ->
+     exists (q:string), x%string=@^(proc_name ++ "_data"++q).
+Proof.
+    intros.
+    unfold Debug.debug_csr_data in H.
+    simpl in H. 
+    inversion H; subst; clear H.
+    + simpl.
+      eapply ex_intro.
+      rewrite ?string_append_assoc.
+      simpl.
+      apply <- string_equal_prefix.
+      econstructor.
+    + inversion H0.
+Qed.
+
+Theorem debug_csr_data_seq_disjoint: forall x n m,
+  In x 
+      (map fst
+         (concat
+            (map csr_reg_csr_field
+               (concat
+                  (map csrViewFields
+                     (concat
+                        (map csrViews
+                           (map Debug.debug_csr_data
+                              (seq m n))))))))) ->
+  exists (q:string), x%string=@^(proc_name ++ "_data" ++q).
+Proof.
+     induction n.
+     + intros.
+       simpl in H.
+       inversion H.
+     + intros.
+       simpl in H.
+       inversion H; subst; clear H.
+       - eapply ex_intro.
+         rewrite ?string_append_assoc.
+         simpl.
+         apply <- string_equal_prefix.
+         econstructor.
+       - eapply IHn.
+         apply H0.
+Qed.*)
 
 Theorem DisjKey_getAllRegisters_intRegFile_csr_regs_debug_csrs:
   DisjKey (getAllRegisters (BaseRegFile intRegFile)) (csr_regs debug_csrs).
@@ -551,8 +602,21 @@ Theorem DisjKey_getAllRegisters_intRegFile_csr_regs_debug_csrs:
   autorewrite with kami_rewrite_db.
   autorewrite with simp_csrs.
   apply DisjKey_NubBy2.
-  unfold debug_csrs_num_data.*)
-
+  unfold debug_csrs_num_data.
+  simpl.
+  autorewrite with simp_csrs.
+  autorewrite with kami_rewrite_db.
+  rewrite ?map_app.
+  simpl.
+  rewrite ?in_app.
+  split.
+  + intro X.
+    inversion X; subst; clear X.
+    - apply debug_csr_data_seq_disjoint in H.
+      inversion H; subst; clear H.
+      simpl in H0.
+      apply string_equal_prefix in H0.
+      inversion H0; subst; clear H0.*)
 
 
 Admitted.
@@ -563,12 +627,7 @@ Theorem DisjKey_getAllMethods_intRegFile_floatRegFile:
   DisjKey (getAllMethods (BaseRegFile intRegFile))
     (getAllMethods (BaseRegFile floatRegFile)).
 Proof.
-    unfold intRegFile.
-    unfold memReservationRegFile.
-    unfold getAllRegisters.
-    unfold getRegisters.
-    unfold getRegFileRegisters.
-    DisjKey_solve.
+    discharge_DisjKey.
 Qed.
 
 Hint Resolve DisjKey_getAllMethods_intRegFile_floatRegFile : wfMod_ConcatMod_Helper.
@@ -577,12 +636,7 @@ Theorem DisjKey_getAllMethods_intRegFile_memReservationRegFile:
   DisjKey (getAllMethods (BaseRegFile intRegFile))
     (getAllMethods (BaseRegFile memReservationRegFile)).
 Proof.
-    unfold intRegFile.
-    unfold memReservationRegFile.
-    unfold getAllRegisters.
-    unfold getRegisters.
-    unfold getRegFileRegisters.
-    DisjKey_solve.
+    discharge_DisjKey.
 Qed.
 
 Hint Resolve DisjKey_getAllMethods_intRegFile_memReservationRegFile : wfMod_ConcatMod_Helper.
@@ -599,7 +653,7 @@ Hint Resolve DisjKey_getAllMethods_intRegFile_mem_device_files_mem_devices : wfM
 Theorem WfMod_intRegFile:
   WfMod (BaseRegFile intRegFile).
 Proof.
-    WfMod_Solve.
+   discharge_wf.
 Qed.
 
 Hint Resolve WfMod_intRegFile : wfMod_ConcatMod_Helper.
@@ -668,10 +722,7 @@ Theorem WFConcat1:
              (map (fun m : RegFileBase => Base (BaseRegFile m))
                 (mem_device_files mem_devices))))).
 Proof.
-    intros.
-    simpl.
-    unfold intRegFile in H.
-    WfConcatAction_Solve.
+    discharge_wf.
 Qed.
 
 Hint Resolve WFConcat1 : wfMod_ConcatMod_Helper.
@@ -709,12 +760,7 @@ Theorem DisjKey_getAllRegisters_floatRefFile_memReservationRegFile:
   DisjKey (getAllRegisters (BaseRegFile floatRegFile))
     (getAllRegisters (BaseRegFile memReservationRegFile)).
 Proof.
-    unfold floatRegFile.
-    unfold memReservationRegFile.
-    unfold getAllRegisters.
-    unfold getRegisters.
-    unfold getRegFileRegisters.
-    DisjKey_solve.
+    discharge_DisjKey.
 Qed.
 
 Hint Resolve DisjKey_getAllRegisters_floatRefFile_memReservationRegFile : wfMod_ConcatMod_Helper.
@@ -739,12 +785,7 @@ Theorem DisjKey_getAllMethods_floatRegFile_memReservationRegFile:
   DisjKey (getAllMethods (BaseRegFile floatRegFile))
     (getAllMethods (BaseRegFile memReservationRegFile)).
 Proof.
-    unfold floatRegFile.
-    unfold memReservationRegFile.
-    unfold getAllRegisters.
-    unfold getRegisters.
-    unfold getRegFileRegisters.
-    DisjKey_solve.
+    discharge_DisjKey.
 Qed.
 
 Hint Resolve DisjKey_getAllMethods_floatRegFile_memReservationRegFile : wfMod_ConcatMod_Helper.
@@ -775,7 +816,7 @@ Theorem WFConcat4:
           (map (fun m : RegFileBase => Base (BaseRegFile m))
              (mem_device_files mem_devices)))).
 Proof.
-    WfConcatAction_Solve.
+    discharge_wf.
 Qed.
 
 Hint Resolve WFConcat4 : wfMod_ConcatMod_Helper.
@@ -783,7 +824,7 @@ Hint Resolve WFConcat4 : wfMod_ConcatMod_Helper.
 Theorem wfMod_floatRegFile:
   WfMod (BaseRegFile floatRegFile).
 Proof.
-    WfMod_Solve.
+    discharge_wf.
 Qed.
 
 Hint Resolve wfMod_floatRegFile : wfMod_ConcatMod_Helper.
@@ -852,39 +893,14 @@ Opaque Nat.mul.
 
 Theorem WfMod_memReservationFile:
   WfMod (BaseRegFile memReservationRegFile).
-Admitted.
-(*Proof.
+(*Admitted.*)
+Proof.
   unfold memReservationRegFile.
   apply BaseWf.
   unfold WfBaseModule.
-  split.
-  intros.
-  simpl in H.
-  inversion H.
-  split.
-  intros.
-  simpl in H.
-  simpl.
+  discharge_wf.
+Qed.
 
-  split.
-
-  apply BaseWf.
-  simpl in H.
-
-  WfMod_Solve.
-
-
-  split.
-  + intros.
-    simpl in H.
-    inversion H.
-  + split.
-    - intros.
-      unfold getMethods in H.
-      unfold getRegFileMethods in H.
-      unfold writeRegFileFn in H.
-      simpl.
-*)
 Hint Resolve WfMod_memReservationFile : wfMod_ConcatMod_Helper.
 
 Theorem WfMod_processorCore_mem_devices:  
@@ -951,23 +967,7 @@ Lemma WfModProcessor:
       autorewrite with kami_rewrite_db.
       rewrite ?map_app.
 
-      repeat ltac_wfMod_ConcatMod.
-
-      repeat (decide equality).
-      repeat (decide equality).
-      repeat (decide equality).
-      repeat (decide equality).
-      repeat (decide equality).
-      repeat (decide equality).
-      repeat (decide equality).
-      repeat (decide equality).
-      repeat (decide equality).
-      repeat (decide equality).
-      repeat (decide equality).
-      repeat (decide equality).
-      repeat (decide equality).
-      repeat (decide equality).
-      repeat (decide equality).
+      repeat ltac_wfMod_ConcatMod;try apply string_dec.
 Qed.
  
 Close Scope kami_expr.
